derived_many1.thy
@@ -4,12 +4,37 @@ theory derived_many1
           derived_then
 begin
 
+\<comment> \<open>Seems like we might want a fallible transform here\<close>
 definition many1 :: "'\<alpha> bidef \<Rightarrow> '\<alpha> list bidef" where
   "many1 a = transform
-                (\<lambda> r rs. r#rs) \<comment> \<open>pair to list\<close>
-                undefined \<comment> \<open>list to pair\<close>
+                (\<lambda> (r, rs). r#rs) \<comment> \<open>pair to list\<close>
+                (\<lambda> l. if l = [] then undefined else (hd l, tl l)) \<comment> \<open>list to pair\<close>
                 (b_then a (many a)) \<comment> \<open>pair parser\<close>
-
 "
+
+
+
+\<comment> \<open>NER\<close>
+lemma many1_is_nonterm[NER_simps]:
+  "is_nonterm (parse (many1 a)) i \<longleftrightarrow> is_nonterm (parse a) i \<or> (\<exists>r l. has_result (parse a) i r l \<and> is_nonterm (parse (many a)) l)"
+  by (simp add: many1_def NER_simps)
+
+lemma many1_is_error[NER_simps]:
+  "is_error (parse (many1 a)) i \<longleftrightarrow> is_error (parse a) i"
+  by (simp add: many1_def NER_simps)
+
+lemma many1_has_result[NER_simps]:
+  "has_result (parse (many1 a)) i r l \<longleftrightarrow> r \<noteq> [] \<and> (\<exists> l'. has_result (parse a) i (hd r) l' \<and> has_result (parse (many a)) l' (tl r) l)"
+  apply (clarsimp simp add: many1_def NER_simps)
+  by fastforce
+
+
+
+\<comment> \<open>FP ner\<close>
+lemma many1_p_is_error[NER_simps]:
+  ""
+
+
+
 
 end
